refactor: remove some useless `bytes` parameter

src/DY.Lib.State.PKI.fst
@@ -10,15 +10,17 @@ open DY.Lib.State.Map
 
 (*** PKI types & invariants ***)
 
-type public_key_type (bytes:Type0) {|bytes_like bytes|} =
-  | PkEnc: [@@@ with_parser #bytes ps_string] usage:string -> public_key_type bytes
-  | Verify: [@@@ with_parser #bytes ps_string] usage:string -> public_key_type bytes
+[@@ with_bytes bytes]
+type public_key_type =
+  | PkEnc: [@@@ with_parser #bytes ps_string] usage:string -> public_key_type
+  | Verify: [@@@ with_parser #bytes ps_string] usage:string -> public_key_type
 
 %splice [ps_public_key_type] (gen_parser (`public_key_type))
 %splice [ps_public_key_type_is_well_formed] (gen_is_well_formed_lemma (`public_key_type))
 
-type pki_key (bytes:Type0) {|bytes_like bytes|} = {
-  ty:public_key_type bytes;
+[@@ with_bytes bytes]
+type pki_key = {
+  ty:public_key_type;
   who:principal;
 }
 
@@ -34,7 +36,7 @@ type pki_value (bytes:Type0) {|bytes_like bytes|} = {
 
 val pki_types: map_types bytes
 let pki_types = {
-  key = pki_key bytes;
+  key = pki_key;
   ps_key = ps_pki_key;
   value = pki_value bytes;
   ps_value = ps_pki_value;
@@ -42,7 +44,7 @@ let pki_types = {
 
 val is_public_key_for:
   crypto_invariants -> trace ->
-  bytes -> public_key_type bytes -> principal -> prop
+  bytes -> public_key_type -> principal -> prop
 let is_public_key_for cinvs tr pk pk_type who =
     match pk_type with
     | PkEnc usg -> (
@@ -73,11 +75,11 @@ let has_pki_invariant pr =
 val initialize_pki: prin:principal -> crypto nat
 let initialize_pki = initialize_map pki_types pki_label
 
-val install_public_key: principal -> nat -> public_key_type bytes -> principal -> bytes -> crypto (option unit)
+val install_public_key: principal -> nat -> public_key_type -> principal -> bytes -> crypto (option unit)
 let install_public_key prin sess_id pk_type who pk =
   add_key_value pki_types pki_label prin sess_id ({ty = pk_type; who;}) ({public_key = pk;})
 
-val get_public_key: principal -> nat -> public_key_type bytes -> principal -> crypto (option bytes)
+val get_public_key: principal -> nat -> public_key_type -> principal -> crypto (option bytes)
 let get_public_key prin sess_id pk_type who =
   let*? res = find_value pki_types pki_label prin sess_id ({ty = pk_type; who;}) in
   return (Some res.public_key)
@@ -101,7 +103,7 @@ let initialize_pki_invariant invs prin tr = ()
 
 val install_public_key_invariant:
   invs:protocol_invariants ->
-  prin:principal -> sess_id:nat -> pk_type:public_key_type bytes -> who:principal -> pk:bytes -> tr:trace ->
+  prin:principal -> sess_id:nat -> pk_type:public_key_type -> who:principal -> pk:bytes -> tr:trace ->
   Lemma
   (requires
     is_public_key_for invs.crypto_invs tr pk pk_type who /\
@@ -119,7 +121,7 @@ let install_public_key_invariant invs prin sess_id pk_type who pk tr = ()
 
 val get_public_key_invariant:
   invs:protocol_invariants ->
-  prin:principal -> sess_id:nat -> pk_type:public_key_type bytes -> who:principal -> tr:trace ->
+  prin:principal -> sess_id:nat -> pk_type:public_key_type -> who:principal -> tr:trace ->
   Lemma
   (requires
     trace_invariant invs tr /\
