src/DY.Lib.State.PrivateKeys.fst
@@ -10,9 +10,10 @@ open DY.Lib.State.Map
 
 (*** Private keys types & invariants ***)
 
-type private_key_type (bytes:Type0) {|bytes_like bytes|} =
-  | PkDec: [@@@with_parser #bytes ps_string] usage:string -> private_key_type bytes
-  | Sign: [@@@with_parser #bytes ps_string] usage:string -> private_key_type bytes
+[@@ with_bytes bytes]
+type private_key_type =
+  | PkDec: [@@@with_parser #bytes ps_string] usage:string -> private_key_type
+  | Sign: [@@@with_parser #bytes ps_string] usage:string -> private_key_type
 
 %splice [ps_private_key_type] (gen_parser (`private_key_type))
 %splice [ps_private_key_type_is_well_formed] (gen_is_well_formed_lemma (`private_key_type))
@@ -26,7 +27,7 @@ type private_key_value (bytes:Type0) {|bytes_like bytes|} = {
 
 val private_keys_types: map_types bytes
 let private_keys_types = {
-  key = private_key_type bytes;
+  key = private_key_type;
   ps_key = ps_private_key_type;
   value = private_key_value bytes;
   ps_value = ps_private_key_value;
@@ -34,7 +35,7 @@ let private_keys_types = {
 
 val is_private_key_for:
   crypto_invariants -> trace ->
-  bytes -> private_key_type bytes -> principal -> prop
+  bytes -> private_key_type -> principal -> prop
 let is_private_key_for cinvs tr sk sk_type who =
     match sk_type with
     | PkDec usg -> (
@@ -61,7 +62,7 @@ let has_private_keys_invariant pr =
   has_map_session_invariant private_keys_pred private_keys_label pr
 
 val private_key_type_to_usage:
-  private_key_type bytes ->
+  private_key_type ->
   usage
 let private_key_type_to_usage sk_type =
   match sk_type with
@@ -73,12 +74,12 @@ let private_key_type_to_usage sk_type =
 val initialize_private_keys: prin:principal -> crypto nat
 let initialize_private_keys = initialize_map private_keys_types private_keys_label
 
-val generate_private_key: principal -> nat -> private_key_type bytes -> crypto (option unit)
+val generate_private_key: principal -> nat -> private_key_type -> crypto (option unit)
 let generate_private_key prin sess_id sk_type =
   let* sk = mk_rand (private_key_type_to_usage sk_type) (principal_label prin) 64 in //TODO
   add_key_value private_keys_types private_keys_label prin sess_id sk_type ({private_key = sk;})
 
-val get_private_key: principal -> nat -> private_key_type bytes -> crypto (option bytes)
+val get_private_key: principal -> nat -> private_key_type -> crypto (option bytes)
 let get_private_key prin sess_id sk_type =
   let*? res = find_value private_keys_types private_keys_label prin sess_id sk_type in
   return (Some res.private_key)
@@ -102,7 +103,7 @@ let initialize_private_keys_invariant invs prin tr = ()
 
 val generate_private_key_invariant:
   invs:protocol_invariants ->
-  prin:principal -> sess_id:nat -> sk_type:private_key_type bytes -> tr:trace ->
+  prin:principal -> sess_id:nat -> sk_type:private_key_type -> tr:trace ->
   Lemma
   (requires
     trace_invariant invs tr /\
@@ -119,7 +120,7 @@ let generate_private_key_invariant invs prin sess_id sk_type tr = ()
 
 val get_private_key_invariant:
   invs:protocol_invariants ->
-  prin:principal -> sess_id:nat -> pk_type:private_key_type bytes -> tr:trace ->
+  prin:principal -> sess_id:nat -> pk_type:private_key_type -> tr:trace ->
   Lemma
   (requires
     trace_invariant invs tr /\
